Minor fixes to CPP 2021 paper/theories

graalir2/Canonicalization.thy
@@ -20,8 +20,6 @@ lemma eval_add_node:
   using eval.AddNode x y by blast
 
 lemma add_const_nodes:
-  assumes det: "\<forall>g m x n v1 v2. 
-    (g m \<turnstile> x n \<mapsto> v1) \<and> (g m \<turnstile> x n \<mapsto> v2) \<longrightarrow> v1 = v2"
   assumes xn: "kind g x = ConstantNode xv"
   assumes yn: "kind g y = ConstantNode yv"
   assumes zn: "kind g z = AddNode x y"
@@ -34,13 +32,13 @@ proof -
     using eval.AddNode eval_const_node xn yn zn by simp
   have wv: "g m \<turnstile> w (kind g w) \<mapsto> IntVal(xv+yv)"
     using eval_const_node wn by auto
-  show ?thesis using det zv wv
+  show ?thesis using evalDet zv wv
     using ew ez by blast
 qed
 
 text_raw \<open>\snip{CreateAddNode}{\<close>
-fun create_add_node :: "IRGraph \<Rightarrow> ID \<Rightarrow> ID \<Rightarrow> IRNode" where 
-  "create_add_node g x y = 
+fun create_add :: "IRGraph \<Rightarrow> ID \<Rightarrow> ID \<Rightarrow> IRNode" where 
+  "create_add g x y = 
     (case kind g x of 
       ConstantNode xv \<Rightarrow> 
         (case kind g y of
@@ -61,10 +59,8 @@ lemma add_node_create:
   assumes yn: "yn = kind g y"
   assumes xv: "g m \<turnstile> x xn \<mapsto> IntVal(xv)"
   assumes yv: "g m \<turnstile> y yn \<mapsto> IntVal(yv)"
-  assumes det: "\<forall>g m x n v1 v2. 
-    (g m \<turnstile> x n \<mapsto> v1) \<and> (g m \<turnstile> x n \<mapsto> v2) \<longrightarrow> v1 = v2"
   shows "(g m \<turnstile> nid (AddNode x y) \<mapsto> IntVal(xv+yv)) \<and>
-  (g m \<turnstile> nid (create_add_node g x y) \<mapsto> IntVal(xv+yv))"
+  (g m \<turnstile> nid (create_add g x y) \<mapsto> IntVal(xv+yv))"
 text_raw \<open>}%endsnip\<close>
 proof -
   have ae: "g m \<turnstile> nid (AddNode x y) \<mapsto> IntVal(xv+yv)"
@@ -73,23 +69,23 @@ proof -
     using eval.RefNode xn xv by blast 
   have refy: "g m \<turnstile> zy (RefNode y) \<mapsto> IntVal yv"
     using eval.RefNode yn yv by blast 
-  have ce: "g m \<turnstile> nid (create_add_node g x y) \<mapsto> IntVal(xv+yv)"
+  have ce: "g m \<turnstile> nid (create_add g x y) \<mapsto> IntVal(xv+yv)"
   proof (cases "kind g x  = ConstantNode xvv")
     case xvvn: True
     have xvv: "xvv = xv" 
-      using ConstantNode det xn xv eval.ConstantNode xvvn by fastforce 
+      using ConstantNode evalDet xn xv eval.ConstantNode xvvn by fastforce 
     thus ?thesis 
     proof (cases "kind g y = ConstantNode yvv")
       case True
       have yvv: "yvv = yv"
-        using ConstantNode det yn yv eval.ConstantNode True by fastforce
+        using ConstantNode evalDet yn yv eval.ConstantNode True by fastforce
       then show ?thesis
       proof -
         have xvv_yvv: "g m \<turnstile> nid (ConstantNode (xvv+yvv)) \<mapsto> IntVal(xv+yv)"
           by (simp add: eval.ConstantNode xvv yvv) 
-        have c_xvv_yvv: "create_add_node g x y = ConstantNode (xvv+yvv)" 
+        have c_xvv_yvv: "create_add g x y = ConstantNode (xvv+yvv)" 
           using xvvn True by simp  
-        have cv1: "g m \<turnstile> nid (create_add_node g x y) \<mapsto> IntVal(xv+yv)"
+        have cv1: "g m \<turnstile> nid (create_add g x y) \<mapsto> IntVal(xv+yv)"
           using c_xvv_yvv xvv_yvv by simp
         then show ?thesis by blast 
       qed
@@ -97,7 +93,7 @@ proof -
       case False
       then show ?thesis
       proof -
-        have cv2: "create_add_node g x y = (if xvv = 0 then RefNode y else AddNode x y)"
+        have cv2: "create_add g x y = (if xvv = 0 then RefNode y else AddNode x y)"
         proof (cases "xvv = 0")
           case True
           then show ?thesis 
@@ -116,14 +112,14 @@ proof -
     proof (cases "kind g y = ConstantNode yvv")
       case True
       have yvv: "yvv = yv"
-        using ConstantNode True det yn yv eval.ConstantNode by fastforce 
-      have cv3: "create_add_node g x y = (if yvv = 0 then RefNode x else AddNode x y)"
+        using ConstantNode True evalDet yn yv eval.ConstantNode by fastforce 
+      have cv3: "create_add g x y = (if yvv = 0 then RefNode x else AddNode x y)"
         using xnotconst True
         sorry
       then show ?thesis using cv3 ae yvv xn xv eval.RefNode by auto
     next 
       case False
-      have cv4: "create_add_node g x y = AddNode x y"
+      have cv4: "create_add g x y = AddNode x y"
         using xnotconst False 
         sorry
       thus ?thesis using cv4 ae by simp
@@ -134,9 +130,9 @@ proof -
 qed
 
 text_raw \<open>\snip{CreateIfNode}{\<close>
-fun create_if_node :: "IRGraph \<Rightarrow> ID \<Rightarrow> ID \<Rightarrow> ID \<Rightarrow> IRNode"
+fun create_if :: "IRGraph \<Rightarrow> ID \<Rightarrow> ID \<Rightarrow> ID \<Rightarrow> IRNode"
   where 
-  "create_if_node g cond tb fb = 
+  "create_if g cond tb fb = 
     (case kind g cond of 
       ConstantNode condv \<Rightarrow> 
         RefNode (if (val_to_bool condv) then tb else fb) |
@@ -206,9 +202,7 @@ lemma if_node_create:
   assumes cv_wf: "g m \<turnstile> cond (kind g cond) \<mapsto> IntVal cv"
   assumes fresh: "nid |\<notin>| fmdom g" 
   assumes gif: "gif = fmupd nid (IfNode cond tb fb) g"
-  assumes gcreate: "gcreate = fmupd nid (create_if_node g cond tb fb) g"
-  assumes det: "\<forall>g m x n v1 v2. 
-    (g m \<turnstile> x n \<mapsto> v1) \<and> (g m \<turnstile> x n \<mapsto> v2) \<longrightarrow> v1 = v2"
+  assumes gcreate: "gcreate = fmupd nid (create_if g cond tb fb) g"
   shows "\<exists>nid'. (gif m \<turnstile> nid \<leadsto> nid') \<and> 
                 (gcreate m \<turnstile> nid \<leadsto> nid')"
 text_raw \<open>}%endsnip\<close>
@@ -228,9 +222,9 @@ proof (cases "kind g cond = ConstantNode val")
     qed
     have create_step: "gcreate \<turnstile> (nid,m) \<rightarrow> (if val_to_bool val then tb else fb,m)"
     proof -
-      have create_kind: "kind gcreate nid = create_if_node g cond tb fb"
+      have create_kind: "kind gcreate nid = create_if g cond tb fb"
         using gcreate by simp
-      have create_fun: "create_if_node g cond tb fb = RefNode (if val_to_bool val then tb else fb)"
+      have create_fun: "create_if g cond tb fb = RefNode (if val_to_bool val then tb else fb)"
         using True create_kind by simp 
       show ?thesis using step.RefNode create_kind create_fun if_cv 
         by simp
@@ -279,7 +273,7 @@ qed
       (ConstantNode xv) \<Rightarrow>
         (case (kind g y) of
           (ConstantNode yv) \<Rightarrow> (add_node g (ConstantNode (xv+yv))) |
-          _ \<Rightarrow> (create_add_node g y x)
+          _ \<Rightarrow> (create_add g y x)
         ) |
       _ \<Rightarrow> 
         (case (kind g y) of
